new/make_array_naive.v
@@ -3,7 +3,7 @@ Require Import Arith Arith.Even Arith.Div2 List.
 Require Import Program.
 Require Import Omega.
 
-Inductive MakeArrayNaiveR : list A -> bin_tree -> nat -> Prop :=
+Inductive MakeArrayNaiveR {A:Set} : list A -> @bin_tree A -> nat -> Prop :=
 | MALR_zero :
     MakeArrayNaiveR nil bt_mt 0
 | MALR_succ :
@@ -14,23 +14,23 @@ Inductive MakeArrayNaiveR : list A -> bin_tree -> nat -> Prop :=
 Hint Constructors MakeArrayNaiveR.
 
 Theorem MakeArrayNaiveR_SequenceR :
-  forall xs bt n,
+  forall A xs (bt:@bin_tree A) n,
     MakeArrayNaiveR xs bt n ->
     SequenceR bt xs.
 Proof.
-  intros xs bt n MALR.
+  intros A xs bt n MALR.
   induction MALR; eauto.
   eapply InsertR_SequenceR; eauto.
 Qed.
 Hint Resolve MakeArrayNaiveR_SequenceR.
 
 Theorem make_array_naive :
-  forall xs,
-    { bt | exists n, MakeArrayNaiveR xs bt n }.
+  forall A xs,
+    { bt : @bin_tree A | exists n, MakeArrayNaiveR xs bt n }.
 Proof.
   induction xs as [| x xs]; [eauto |].
   destruct IHxs as [bt IR].
-  remember (insert x bt).
+  remember (insert A x bt).
   clear Heqs.
   destruct s as [bt' insIR'].
   exists bt'.
@@ -41,11 +41,11 @@ Proof.
 Defined.
 
 Theorem MakeArrayNaiveR_Braun :
-  forall xs bt n,
+  forall A xs (bt:@bin_tree A) n,
     MakeArrayNaiveR xs bt n ->
     Braun bt (length xs).
 Proof.
-  intro xs.
+  intros A xs.
   induction xs as [| x xs]; intros bt n MkArrR.
 
   simpl.
@@ -54,14 +54,14 @@ Proof.
 
   simpl.
   inversion_clear MkArrR.
-  apply (InsertR_Braun x (length xs) insert_time bt0).
+  apply (InsertR_Braun A x (length xs) insert_time bt0).
   apply (IHxs bt0 time H0).
   assumption.
 Qed.
 Hint Resolve MakeArrayNaiveR_Braun.
 
 Theorem MakeArrayNaiveR_correct :
-  forall xs bt n,
+  forall A xs (bt:@bin_tree A) n,
     MakeArrayNaiveR xs bt n ->
     forall i x,
       IndexR bt i x ->
@@ -107,16 +107,16 @@ Qed.
 Hint Resolve man_time_nlogn.
 
 Theorem MakeArrayNaiveR_time :
-  forall xs bt t,
+  forall A xs (bt:@bin_tree A) t,
     MakeArrayNaiveR xs bt t ->
     t = man_time (length xs).
 Proof.
-  intros xs bt t MALR.
+  intros A xs bt t MALR.
   induction MALR; eauto.
   rename H into IR.
   subst.
   apply MakeArrayNaiveR_Braun in MALR.
-  eapply (InsertR_time _ _ _ _ _ MALR) in IR.
+  eapply (InsertR_time _ _ _ _ _ _ MALR) in IR.
   subst.
   replace (fl_log (length xs) + 1) with (cl_log (length (x :: xs))).
   auto.
@@ -127,10 +127,10 @@ Qed.
 Hint Rewrite MakeArrayNaiveR_time.
 
 Theorem MakeArrayNaiveR_bound :
-  forall xs bt t,
+  forall A xs (bt:@bin_tree A) t,
     MakeArrayNaiveR xs bt t ->
     t <= (length xs) * cl_log (length xs).
 Proof.
-  intros xs bt t MALR.
-  rewrite (MakeArrayNaiveR_time xs bt t); eauto.
+  intros A xs bt t MALR.
+  rewrite (MakeArrayNaiveR_time A xs bt t); eauto.
 Qed.
