new/make_array_td.v
@@ -3,7 +3,7 @@ Require Import Arith Arith.Even Arith.Div2 List.
 Require Import Program.
 Require Import Omega.
 
-Inductive UnravelR : list A -> list A -> list A -> nat -> Prop :=
+Inductive UnravelR {A:Set} : list A -> list A -> list A -> nat -> Prop :=
 | UR_nil :
     UnravelR nil nil nil 0
 | UR_cons :
@@ -13,11 +13,11 @@ Inductive UnravelR : list A -> list A -> list A -> nat -> Prop :=
 Hint Constructors UnravelR.
 
 Lemma UnravelR_interleave :
-  forall xs evens odds ut,
-    UnravelR xs evens odds ut ->
+  forall A xs evens odds ut,
+    @UnravelR A xs evens odds ut ->
     xs = interleave evens odds.
 Proof.
-  intros xs evens odds ut UR.
+  intros A xs evens odds ut UR.
   induction UR.
 
   auto.
@@ -27,55 +27,55 @@ Qed.
 Hint Rewrite UnravelR_interleave.
 
 Lemma UnravelR_length_both :
-  forall xs evens odds ut,
-    UnravelR xs evens odds ut ->
+  forall A xs evens odds ut,
+    @UnravelR A xs evens odds ut ->
     length evens < S (length xs)
  /\ length odds < S (length xs).
 Proof.
-  intros xs evens odds ut UR.
+  intros A xs evens odds ut UR.
   induction UR; simpl; omega.
 Qed.
 Hint Resolve UnravelR_length_both.
 
 Lemma UnravelR_length_evens :
-  forall xs evens odds ut,
-    UnravelR xs evens odds ut ->
+  forall A xs evens odds ut,
+    @UnravelR A xs evens odds ut ->
     length evens < S (length xs).
 Proof.
-  intros xs evens odds ut UR.
+  intros A xs evens odds ut UR.
   eapply UnravelR_length_both in UR.
   tauto.
 Qed.
 Hint Resolve UnravelR_length_evens.
 
 Lemma UnravelR_length_odds :
-  forall xs evens odds ut,
-    UnravelR xs evens odds ut ->
+  forall A xs evens odds ut,
+    @UnravelR A xs evens odds ut ->
     length odds < S (length xs).
 Proof.
-  intros xs evens odds ut UR.
+  intros A xs evens odds ut UR.
   eapply UnravelR_length_both in UR.
   tauto.
 Qed.
 Hint Resolve UnravelR_length_odds.
 
 Lemma UnravelR_length :
-  forall xs evens odds ut,
-    UnravelR xs evens odds ut ->
+  forall A xs evens odds ut,
+    @UnravelR A xs evens odds ut ->
     length odds <= length evens <= length odds + 1.
 Proof.
-  intros xs evens odds ut UR.
+  intros A xs evens odds ut UR.
   induction UR; simpl; omega.
 Qed.
 Hint Resolve UnravelR_length.
 
 Theorem unravel :
-  forall xs,
-    { eo | exists t, UnravelR xs (fst eo) (snd eo) t }.
+  forall A xs,
+    { eo | exists t, @UnravelR A xs (fst eo) (snd eo) t }.
 Proof.
   induction xs as [|x xs].
 
-  exists (@nil A, @nil A).
+  exists (@nil A, @nil A). simpl.
   eauto.
 
   destruct IHxs as [[odds evens] UR].
@@ -86,16 +86,16 @@ Proof.
 Defined.
 
 Theorem UnravelR_time :
-  forall xs evens odds ut,
-    UnravelR xs evens odds ut ->
+  forall A xs evens odds ut,
+    @UnravelR A xs evens odds ut ->
     ut = length xs.
 Proof.
-  intros xs evens odds ut UR.
+  intros A xs evens odds ut UR.
   induction UR; simpl; try omega.
 Qed.
 Hint Rewrite UnravelR_time.
 
-Inductive MakeArrayTDR : list A -> bin_tree -> nat -> Prop :=
+Inductive MakeArrayTDR {A:Set} : list A -> @bin_tree A -> nat -> Prop :=
 | MATDR_zero :
     MakeArrayTDR nil bt_mt 0
 | MATDR_succ :
@@ -108,11 +108,11 @@ Inductive MakeArrayTDR : list A -> bin_tree -> nat -> Prop :=
 Hint Constructors MakeArrayTDR.
 
 Theorem MakeArrayTDR_SequenceR :
-  forall xs bt n,
+  forall A xs (bt:@bin_tree A) n,
     MakeArrayTDR xs bt n ->
     SequenceR bt xs.
 Proof.
-  intros xs bt n MAR.
+  intros A xs bt n MAR.
   induction MAR; eauto.
   rename H into UR.
   apply UnravelR_interleave in UR.
@@ -122,14 +122,14 @@ Qed.
 Hint Resolve MakeArrayTDR_SequenceR.
 
 Lemma make_array_td_base :
-  forall xs,
-    (forall ys, length ys < length xs ->
+  forall (A:Set) (xs:list A),
+    (forall (ys:list A), length ys < length xs ->
                 { bt | exists t, MakeArrayTDR ys bt t }) ->
     { bt | exists t, MakeArrayTDR xs bt t }.
 Proof.
-  intros [|x xs] IH.
+  intros A [|x xs] IH.
   eauto.
-  destruct (unravel xs) as [[evens odds] UR].
+  destruct (unravel A xs) as [[evens odds] UR].
   simpl in UR.
   destruct (IH evens) as [s MARs].
    simpl. destruct UR as [t UR]. eauto.
@@ -148,10 +148,10 @@ be to figure out how to generate the IH that make_array_td_base needs
 directly. *)
 
 Theorem make_array_td :
-  forall xs,
-    { bt | exists t, MakeArrayTDR xs bt t }.
+  forall A xs,
+    { bt : @bin_tree A | exists t, MakeArrayTDR xs bt t }.
 Proof.
-  intros xs.
+  intros A xs.
   remember (length xs).
   generalize n xs Heqn. clear n xs Heqn.
   apply (well_founded_induction_type
@@ -166,11 +166,11 @@ Proof.
 Defined.
 
 Theorem MakeArrayTDR_Braun :
-  forall xs bt n,
+  forall A xs (bt:@bin_tree A) n,
     MakeArrayTDR xs bt n ->
     Braun bt (length xs).
 Proof.
-  intros xs bt n MAR.
+  intros A xs bt n MAR.
   induction MAR; simpl; eauto.
 
   rename H into UR.
@@ -186,7 +186,7 @@ Qed.
 Hint Resolve MakeArrayTDR_Braun.
 
 Theorem MakeArrayTDR_correct :
-  forall xs bt n,
+  forall A xs (bt:@bin_tree A) n,
     MakeArrayTDR xs bt n ->
     forall i x,
       IndexR bt i x ->
@@ -218,17 +218,17 @@ Proof.
 Qed.
 
 Lemma MakeArrayTDR_exact_time :
-  forall xs bt t,
+  forall A xs (bt:@bin_tree A) t,
     MakeArrayTDR xs bt t ->
     t = mat_time (length xs).
 Proof.
-  intros xs bt t MALR.
+  intros A xs bt t MALR.
   induction MALR; eauto.
   rename H into UR.
   replace (length (x :: xs)) with (S (length xs)); eauto.
   subst.
-  rewrite (UnravelR_time _ _ _ _ UR).
-  rewrite (UnravelR_interleave _ _ _ _ UR).
+  rewrite (UnravelR_time _ _ _ _ _ UR).
+  rewrite (UnravelR_interleave _ _ _ _ _ UR).
   assert (length evens <= length odds <= length evens+1) as BTI;
     [eapply UnravelR_length; apply UR|].
   clear MALR1 MALR2 s t x UR xs unravel_time.
@@ -311,7 +311,7 @@ Proof.
 Qed.
 
 Theorem MakeArrayTDR_time :
-  forall xs bt t,
+  forall A xs (bt:@bin_tree A) t,
     MakeArrayTDR xs bt t ->
     t <= (length xs) * cl_log (length xs).
 Proof.
