new/same_structure.v
@@ -5,7 +5,7 @@ Require Import braun util Omega.
 Require Import Program.Equality.
 Set Implicit Arguments.
 
-Inductive same_structure : bin_tree -> bin_tree -> Prop :=
+Inductive same_structure {A:Set} : @bin_tree A -> @bin_tree A -> Prop :=
 | SS_mt :
     same_structure bt_mt bt_mt
 | SS_node :
@@ -17,14 +17,14 @@ Inductive same_structure : bin_tree -> bin_tree -> Prop :=
 Hint Constructors same_structure.
 
 Theorem same_structure_same_size :
-  forall bt1 bt2,
+  forall A (bt1:@bin_tree A) bt2,
     same_structure bt1 bt2 ->
     forall n1 n2,
       Braun bt1 n1 ->
       Braun bt2 n2 ->
       n1 = n2.
 Proof.
-  intros bt1 bt2 SS.
+  intros A bt1 bt2 SS.
   induction SS; intros n1 n2 B1 B2;
   inversion_clear B1;
   inversion_clear B2; eauto.
@@ -32,11 +32,12 @@ Qed.
 Hint Rewrite same_structure_same_size.
 
 Theorem same_size_same_structure :
-  forall n bt1 bt2,
+  forall A n (bt1:@bin_tree A) bt2,
     Braun bt1 n ->
     Braun bt2 n ->
     same_structure bt1 bt2.
 Proof.
+  intros A.
   apply (well_founded_ind
            lt_wf
            (fun n => forall (b1 b2 : bin_tree),
